rework BVL->bytecode
make it compile lists of expressions at a time (to match the BVL
semantics). make it one recursive function rather than a bundle. fix
proper compilation of tail calls. add compilation of most of the
primitive ops. prove an "append_out" theorem about it.

it's likely wrong in various (hopefully) minor ways - still trying to
work out the right correctness theorem statement.

new-backend/bvlBytecodeScript.sml
@@ -1,11 +1,14 @@
 open HolKernel boolLib bossLib lcsymtacs
-open bytecodeTheory bvlTheory
+open listTheory rich_listTheory quantHeuristicsLib quantHeuristicsLibAbbrev arithmeticTheory
+open miscTheory bytecodeTheory bytecodeExtraTheory bvlTheory
 val _ = new_theory"bvlBytecode"
 
 val _ = Datatype`
   bvl_bc_state = <|
     next_label : num;
     out : bc_inst list |>`
+
+val bvl_bc_state_component_equality = theorem"bvl_bc_state_component_equality"
 
 val emit_def = Define`
   emit = FOLDL (λs i. s with <| out := i :: s.out |>)`
@@ -15,6 +18,19 @@ val get_label_def = Define`
 
 val _ = Datatype`
   bvl_bc_tail = TCNonTail | TCTail num num`
+
+val stackshiftaux_def = Define`
+  stackshiftaux (n:num) i j =
+    if n = 0 then []
+    else (Load i)::(Store j)::(stackshiftaux (n-1) (i+1) (j+1))`
+
+val stackshift_def = Define`
+  stackshift j k =
+    if k = 0 then []
+    else if j = 0 then [Pops (k-1); Pop]
+    else if j = 1 then [Pops k]
+    else if j ≤ k then (GENLIST (K (Store (k-1))) j)++(stackshift 0 (k-j))
+    else (stackshiftaux k (j-k) j)++(stackshift (j-k) k)`
 
 val pushret_def = Define`
   (pushret TCNonTail s = s) ∧
@@ -34,61 +50,117 @@ val pushret_def = Define`
       (* v::ret *)
         Return])`
 
-val bvl_bc_def = tDefine "bvl_bc"`
-  (bvl_bc cenv t sz s (Var n) =
+val bvl_bc_def = C (tDefine "bvl_bc")
+  (WF_REL_TAC`measure (bvl_exp1_size o SND o SND o SND o SND)`)`
+  (bvl_bc cenv t sz s [] = s) ∧
+  (bvl_bc cenv t sz s (e1::e2::es) =
+    let s = bvl_bc cenv TCNonTail sz s [e1] in
+    bvl_bc cenv t (sz+1) s (e2::es)) ∧
+  (bvl_bc cenv t sz s [Var n] =
      if n < LENGTH cenv then
        pushret t (emit s [Stack(Load(sz-(EL n cenv)))])
      else s) ∧
-  (bvl_bc cenv t sz s (If e1 e2 e3) =
+  (bvl_bc cenv t sz s [If e1 e2 e3] =
     let (s,l1) = get_label s in
     let (s,l2) = get_label s in
-    let s = bvl_bc cenv TCNonTail sz s e1 in
+    let s = bvl_bc cenv TCNonTail sz s [e1] in
     let s = emit s [JumpIf (Lab l1)] in
-    let s = bvl_bc cenv t sz s e3 in
+    let s = bvl_bc cenv t sz s [e3] in
     let s = emit s [Jump (Lab l2);Label l1] in
-    let s = bvl_bc cenv t sz s e2 in
+    let s = bvl_bc cenv t sz s [e2] in
             emit s [Label l2]) ∧
-  (bvl_bc cenv t sz s (Let es e) =
-    bvl_bc_bindings cenv sz s es t 0 e) ∧
-  (bvl_bc cenv t sz s (Raise e) =
-    let s = bvl_bc cenv TCNonTail sz s e in
+  (bvl_bc cenv t sz s [Let es e] =
+    let s = bvl_bc cenv TCNonTail sz s es in
+    let n = LENGTH es in
+    let s =
+      bvl_bc ((GENLIST (λk. sz+k-n) n)++cenv)
+             (case t of TCTail j k => TCTail j (k+n) | _ => t)
+             (sz+n) s [e] in
+    emit s (case t of TCNonTail => [Stack(Pops n)] | _ => [])) ∧
+  (bvl_bc cenv t sz s [Raise e] =
+    let s = bvl_bc cenv TCNonTail sz s [e] in
             emit s [PopExc; Return]) ∧
-  (bvl_bc cenv t sz s (Handle e1 e2) =
+  (bvl_bc cenv t sz s [Handle e1 e2] =
     let (s,l0) = get_label s in
     let (s,l1) = get_label s in
     let s = emit s [PushPtr (Lab l0); PushExc] in
-    let s = bvl_bc cenv TCNonTail (sz+2) s e1 in
+    let s = bvl_bc cenv TCNonTail (sz+2) s [e1] in
     let s = pushret t (emit s [PopExc; Stack (Pops 1)]) in
     let s = emit s [Jump (Lab l1); Label l0] in
-    let s = bvl_bc ((sz+1)::cenv) t (sz+1) s e2 in
+    let s = bvl_bc ((sz+1)::cenv) t (sz+1) s [e2] in
             emit s [Label l1]) ∧
-  (bvl_bc cenv t sz s (Tick e) =
+  (bvl_bc cenv t sz s [Tick e] =
     let s = emit s [Tick] in
-            bvl_bc cenv t sz s e) ∧
-  (bvl_bc cenv t sz s (Call dest es) =
-    let s = bvl_bc_list cenv sz s es in
+            bvl_bc cenv t sz s [e]) ∧
+  (bvl_bc cenv t sz s [Call dest es] =
+    let s = bvl_bc cenv TCNonTail sz s es in
     let s = emit s [Tick] in
-    case dest of
-    | NONE => emit s [Stack(Load 0); CallPtr]
-    | SOME p => emit s [Stack(PushInt 0); Call (Lab p)]) ∧
-  (bvl_bc cenv t sz s (Op op es) =
-    let s = bvl_bc_list cenv sz s es in
-            pushret t s (* TODO *)) ∧
-  (bvl_bc_list cenv sz s [] = s) ∧
-  (bvl_bc_list cenv sz s (e::es) =
-    let s = bvl_bc cenv TCNonTail sz s e in
-      bvl_bc_list cenv (sz+1) s es) ∧
-  (bvl_bc_bindings cenv sz s [] t n b =
-     case t of
-     | TCNonTail => emit (bvl_bc cenv t sz s b) [Stack (Pops n)]
-     | TCTail j k => bvl_bc cenv (TCTail j (k+n)) sz s b) ∧
-  (bvl_bc_bindings cenv sz s (e::es) t n b =
-     let s = bvl_bc cenv TCNonTail sz s e in
-       bvl_bc_bindings ((sz+1)::cenv) (sz+1) s es t (n+1) b)`
-  (WF_REL_TAC`inv_image ($< LEX $<)
-      (λx. case x of INL (_,_,_,_,e) => (bvl_exp_size e,2:num)
-                   | INR (INL (_,_,_,es)) => (bvl_exp1_size es,1)
-                   | INR (INR (_,_,_,es,_,_,b)) => (bvl_exp1_size (b::es),0))`)
+    let n = LENGTH es in
+    case t of
+    | TCNonTail =>
+        (case dest of
+           (* ptr::args *)
+         | NONE => emit s [Stack(Load 0); CallPtr]
+           (* args *)
+         | SOME p => emit s [Stack(PushInt 0); Call (Lab p)])
+    | TCTail j k =>
+      (* args++|k|++ret::|j| *)
+        (case dest of
+         | NONE =>
+           (* ptr::args++|k|++ret::|j| *)
+             let s = emit s [Stack(Load 0);Stack(Load (1+1+n+k));Stack(Store 1);Stack(PushInt 0)] in
+           (*      ptr::ptr::args++|k|++ret::|j| *)
+           (* ret::ptr::ptr::args++|k|++ret::|j| *)
+           (*      ptr::ret::args++|k|++ret::|j| *)
+           (*  ig::ptr::ret::args++|k|++ret::|j| *)
+             let s = emit s (MAP Stack (stackshift (1+1+1+n) (k+1+j))) in
+           (* ig::ptr::ret::args *)
+                     emit s [Return]
+         | SOME p =>
+           (* args++|k|++ret::|j| *)
+             let s = emit s [Stack(Load(n+k));Stack(PushInt 0)] in
+           (*     ret::args++|k|++ret::|j| *)
+           (* ig::ret::args++|k|++ret::|j| *)
+             let s = emit s (MAP Stack (stackshift (1+1+n) (k+1+j))) in
+           (* ig::ret::args *)
+                     emit s [Jump (Lab p)])) ∧
+  (bvl_bc cenv t sz s [Op op es] =
+    let s = bvl_bc cenv TCNonTail sz s es in
+    let s = emit s (case op of
+    | Global n => [Gread n]
+    | AllocGlobal => [Galloc 1]
+    | SetGlobal n => [Gupdate n]
+    | Cons n => [Stack(PushInt (&(LENGTH es))); Stack (Cons n)]
+    | El n => [Stack (PushInt (&n)); Stack El]
+    | El2 => [Stack El]
+    | LengthBlock => [Stack LengthBlock]
+    | Length => [Length]
+    | LengthByte => [LengthByte]
+    | RefByte => [RefByte]
+    | Ref2 => [Ref]
+    | DerefByte => [DerefByte]
+    | UpdateByte => [UpdateByte]
+    | FromList n => [] (* TODO *)
+    | ToList => [] (* TODO *)
+    | Const i => [Stack (PushInt i)]
+    | TagEq n => [Stack (TagEq n)]
+    | IsBlock => [Stack IsBlock]
+    | Equal => [Stack Equal]
+    | Ref => [] (* TODO *)
+    | Deref => [Deref]
+    | Update => [Update]
+    | Label n => [PushPtr (Lab n)]
+    | Print => [Print]
+    | PrintC c => [PrintC c]
+    | Add => [Stack Add]
+    | Sub => [Stack Sub]
+    | Mult => [Stack Mult]
+    | Div => [Stack Div]
+    | Mod => [Stack Mod]
+    | Less => [Stack Less])
+    in pushret t s)`
+
+val bvl_bc_ind = theorem"bvl_bc_ind"
 
 (*
 stack = a,b,x5,x4,x3,c,x7,x6,d
@@ -121,14 +193,94 @@ val good_env_def = Define`
   good_env sz st =
       LIST_REL (λv n. n ≤ sz ∧ (sz-n) < LENGTH st ∧ (EL (sz-n) st = v))`
 
+val pushret_append_out = store_thm("pushret_append_out",
+  ``∀t s. ((pushret t s).next_label = s.next_label) ∧
+          ∃bc. ((pushret t s).out = bc ++ s.out) ∧
+               (FILTER is_Label bc = [])``,
+  Cases >> rw[pushret_def,emit_def])
+
+val FOLDL_emit_append_out = prove(
+  ``∀ls s. emit s ls = s with out := REVERSE ls ++ s.out``,
+  Induct >> simp[bvl_bc_state_component_equality,emit_def] >> fs[emit_def])
+  |> SIMP_RULE (srw_ss())[]
+
+val bvl_bc_append_out = store_thm("bvl_bc_append_out",
+  ``(∀cenv t sz s e.
+       ∃bc. ((bvl_bc cenv t sz s e).out = bc ++ s.out) ∧
+            ALL_DISTINCT (FILTER is_Label bc) ∧
+            s.next_label ≤ (bvl_bc cenv t sz s e).next_label ∧
+            EVERY (between s.next_label (bvl_bc cenv t sz s e).next_label)
+              (MAP dest_Label (FILTER is_Label bc)))``,
+  ho_match_mp_tac bvl_bc_ind >>
+  strip_tac >- simp[bvl_bc_def] >>
+  strip_tac >- (
+    simp[bvl_bc_def] >> rw[] >>
+    fs[FILTER_APPEND,ALL_DISTINCT_APPEND,EVERY_MAP,MEM_FILTER,EVERY_FILTER,
+       is_Label_rwt,PULL_EXISTS] >>
+    fs[EVERY_MEM,between_def] >> rw[] >> res_tac >> fsrw_tac[ARITH_ss][] >>
+    strip_tac >> res_tac >> fsrw_tac[ARITH_ss][] ) >>
+  strip_tac >- (
+    simp[bvl_bc_def] >> rw[] >>
+    SIMPLE_QUANT_ABBREV_TAC[select_fun_constant``pushret``2"s0"] >>
+    qspecl_then[`t`,`s0`]mp_tac(pushret_append_out) >> rw[] >> fs[Abbr`s0`] >>
+    fs[emit_def,FILTER_APPEND] ) >>
+  strip_tac >- (
+    simp[bvl_bc_def,get_label_def] >> rw[] >>
+    fs[FILTER_APPEND,ALL_DISTINCT_APPEND,EVERY_MAP,MEM_FILTER,EVERY_FILTER,
+       emit_def,is_Label_rwt,PULL_EXISTS] >>
+    fs[EVERY_MEM,between_def] >> rw[] >> res_tac >> fsrw_tac[ARITH_ss][] >>
+    spose_not_then strip_assume_tac >> rw[] >> res_tac >> fsrw_tac[ARITH_ss][]) >>
+  strip_tac >- (
+    simp[bvl_bc_def,emit_def] >> rw[] >>
+    Cases_on`t`>>fs[]>>
+    fs[FILTER_APPEND,ALL_DISTINCT_APPEND,EVERY_MAP,MEM_FILTER,EVERY_FILTER,
+       emit_def,is_Label_rwt,PULL_EXISTS] >>
+    fs[EVERY_MEM,between_def] >> rw[] >> res_tac >> fsrw_tac[ARITH_ss][] >>
+    spose_not_then strip_assume_tac >> rw[] >> res_tac >> fsrw_tac[ARITH_ss][]) >>
+  strip_tac >- (
+    simp[bvl_bc_def,emit_def] >> rw[] >>
+    fs[FILTER_APPEND,ALL_DISTINCT_APPEND,EVERY_MAP,MEM_FILTER,EVERY_FILTER,
+       emit_def,is_Label_rwt,PULL_EXISTS]) >>
+  strip_tac >- (
+    simp[bvl_bc_def,get_label_def,emit_def] >> rw[] >>
+    SIMPLE_QUANT_ABBREV_TAC[select_fun_constant``pushret``2"s0"] >>
+    qspecl_then[`t`,`s0`]mp_tac(pushret_append_out) >> rw[] >> fs[Abbr`s0`] >>
+    fs[FILTER_APPEND,ALL_DISTINCT_APPEND,EVERY_MAP,MEM_FILTER,EVERY_FILTER,
+       is_Label_rwt,PULL_EXISTS] >>
+    fs[EVERY_MEM,between_def] >> rw[] >> res_tac >> fsrw_tac[ARITH_ss][] >>
+    spose_not_then strip_assume_tac >> rw[] >> res_tac >> fsrw_tac[ARITH_ss][] >>
+    fs[FILTER_EQ_NIL,EVERY_MEM,is_Label_rwt] >> res_tac >> fs[]) >>
+  strip_tac >- (
+    simp[bvl_bc_def,emit_def] >> rw[] >>
+    fs[FILTER_APPEND,ALL_DISTINCT_APPEND,EVERY_MAP,MEM_FILTER,EVERY_FILTER,
+       emit_def,is_Label_rwt,PULL_EXISTS]) >>
+  strip_tac >- (
+    simp[bvl_bc_def,emit_def,FOLDL_emit_append_out] >> rw[] >>
+    Cases_on`t`>>Cases_on`dest`>>fs[]>>
+    fs[FILTER_APPEND,ALL_DISTINCT_APPEND,EVERY_MAP,MEM_FILTER,EVERY_FILTER,
+       FILTER_REVERSE,EVERY_REVERSE,ALL_DISTINCT_REVERSE,is_Label_rwt,PULL_EXISTS] >>
+    fs[MEM_MAP] >>
+    qmatch_abbrev_tac`ALL_DISTINCT ls` >>
+    qsuff_tac`ls=[]`>>rw[Abbr`ls`]>>
+    rw[FILTER_EQ_NIL,EVERY_MAP]) >>
+  strip_tac >- (
+    simp[bvl_bc_def] >> rw[] >>
+    Cases_on`op`>>fs[emit_def] >>
+    SIMPLE_QUANT_ABBREV_TAC[select_fun_constant``pushret``2"s0"] >>
+    qspecl_then[`t`,`s0`]mp_tac(pushret_append_out) >> rw[] >> fs[Abbr`s0`] >>
+    fs[FILTER_APPEND,ALL_DISTINCT_APPEND,EVERY_MAP,MEM_FILTER,EVERY_FILTER,
+       is_Label_rwt,PULL_EXISTS] >>
+    fs[EVERY_MEM,between_def] >> rw[] >> res_tac >> fsrw_tac[ARITH_ss][] >>
+    spose_not_then strip_assume_tac >> rw[] >> res_tac >> fsrw_tac[ARITH_ss][] >>
+    fs[FILTER_EQ_NIL,EVERY_MEM,is_Label_rwt] >> res_tac >> fs[]))
+
 (*
 val bvl_bc_correct = store_thm("bvl_bc_correct",
   ``∀exps env s res s' bs1 bc0 code bc1 cenv t sz cs stw ret sp hdl rst.
       (bEval (exps,env,s) = (res,s')) ∧ res ≠ Error ∧
       (good_env sz bs1.stack env cenv) ∧
       (good_code_env s.code bs1.code) ∧
-
-      ((bvl_bc cenv t sz cs exp).out = REVERSE code ++ cs.out) ∧
+      ((bvl_bc cenv t sz cs exps).out = REVERSE code ++ cs.out) ∧
       (bs1.code = bc0 ++ code ++ bc1) ∧
       (bs1.pc = next_addr bs1.inst_length bc0) ∧
       (bs1.clock = SOME s.clock) ∧ (bs1.globals = s.globals) ∧ (bs1.refs = s.refs) ∧
